Uncompiled changes for John.

sel4_artifacts/UxASSeL4/components/Asset_Waypoint_Manager/include/tb_Asset_Waypoint_Manager.h
@@ -48,7 +48,7 @@ void component_entry(const int64_t * periodic_dispatcher);
 
 
  void component_init(const int64_t *arg);
- bool tb_out_waypoint_enqueue(const MissionSoftware__waypoint_impl * tb_out_waypoint);
+ bool tb_out_waypoint_enqueue(const MissionSoftware__mission_command_impl * tb_out_waypoint);
  // reader prototype for tb_in_uart_packet
 bool tb_in_uart_packet_dequeue(SMACCM_DATA__UART_Packet_i * tb_in_uart_packet);
 // user dispatch entrypoints for port tb_in_uart_packet
